isabelle/Util/Serialisation.thy
@@ -1,0 +1,334 @@
+theory Serialisation
+  imports "HOL-Library.Word" ByteString
+begin
+
+fun positiveIntToByteStringAux :: "int \<Rightarrow> 8 word list" where
+"positiveIntToByteStringAux x =
+  (if x < 128 then [word_of_int x] else (word_of_int ((x mod 128) + 128)) # (positiveIntToByteStringAux ((x div 128) - 1)))"
+
+fun positiveIntToByteString :: "int \<Rightarrow> ByteString" where
+"positiveIntToByteString x = ByteString (positiveIntToByteStringAux x)"
+
+fun byteStringToPositiveIntAux :: "8 word list \<Rightarrow> (int \<times> 8 word list) option" where
+"byteStringToPositiveIntAux Nil = None" |
+"byteStringToPositiveIntAux (Cons xw rest) =
+  (let x = uint xw in
+    (if x < 128
+     then (Some (x, rest))
+     else (case byteStringToPositiveIntAux rest of
+             None \<Rightarrow> None
+           | Some (y, extra) \<Rightarrow> Some ((x - 128) + 128 * (y + 1), extra))))"
+
+fun byteStringToPositiveInt :: "ByteString \<Rightarrow> (int \<times> ByteString) option" where
+"byteStringToPositiveInt (ByteString x) =
+   (case byteStringToPositiveIntAux x of
+      Some (y, rest) \<Rightarrow> Some (y, ByteString rest)
+    | None \<Rightarrow> None)"
+
+lemma packByteStringToPositveIntLazy : "(case byteStringToPositiveIntAux (innerListByteString x) of
+                                          Some (y, rest) \<Rightarrow> Some (y, ByteString rest)
+                                        | None \<Rightarrow> None) = byteStringToPositiveInt x"
+  by (metis byteStringToPositiveInt.simps innerListByteString.elims)
+
+lemma smallerIntInductionRestrictedToNat : "(\<And> x :: nat. (\<And> y :: nat . y < x \<Longrightarrow> P (int y)) \<Longrightarrow> P (int x)) \<Longrightarrow> P (int z)"
+  apply (induct rule:Orderings.wellorder_class.less_induct)
+  by auto
+
+lemma smallerIntInduction : "(\<And> x :: int. x \<ge> 0 \<Longrightarrow> (\<And> y :: int . 0 \<le> y \<Longrightarrow> y < x \<Longrightarrow> P y) \<Longrightarrow> P x) \<Longrightarrow> z \<ge> 0 \<Longrightarrow> P z"
+  apply (cases z)
+  subgoal for n
+    
+    by (metis (mono_tags) nat_int nat_less_iff of_nat_0_le_iff smallerIntInductionRestrictedToNat zero_le_imp_eq_int)
+  by linarith
+
+lemma fold_sig_bit_in_word_of_int : "word_of_int (x mod 128) + 128 = word_of_int (x mod 128 + 128)"
+  by auto
+
+lemma distrib_cons_append_bytestrings : "appendByteStrings (consByteString x y) z = consByteString x (appendByteStrings y z)"
+  by (metis appendByteStrings.simps append_Cons byteStringToPositiveInt.cases consByteString.simps)
+
+lemma positiveIntToByteStringToPositiveIntAux_inductionStep : "0 \<le> (x :: int) \<Longrightarrow> (\<And>ya. 0 \<le> ya \<Longrightarrow> ya < x \<Longrightarrow> byteStringToPositiveIntAux ((positiveIntToByteStringAux ya) @ y) = Some (ya, y))
+                                                                    \<Longrightarrow> byteStringToPositiveIntAux ((positiveIntToByteStringAux x) @ y) = Some (x, y)"
+  apply (cases "x < 128")
+  apply (simp add:take_bit_eq_mod intToWordToUint Let_def)
+  apply (simp only:positiveIntToByteStringAux.simps[of x] if_False intToWordToUint)
+  apply (simp del:positiveIntToByteStringAux.simps add:Let_def intToWordToUint )
+  apply (simp only:fold_sig_bit_in_word_of_int intToWordToUint)
+  by simp
+
+
+lemma positiveIntToByteStringToPositiveIntAux : "(x :: int) \<ge> 0 \<Longrightarrow> byteStringToPositiveIntAux ((positiveIntToByteStringAux x) @ y) = Some (x, y)"
+  apply (rule smallerIntInduction[of "\<lambda> x. byteStringToPositiveIntAux (positiveIntToByteStringAux x @ y) = Some (x, y)"])
+  using positiveIntToByteStringToPositiveIntAux_inductionStep apply blast
+  by simp
+
+theorem positiveIntToByteStringToPositiveInt : "(x :: int) \<ge> 0 \<Longrightarrow> byteStringToPositiveInt (appendByteStrings (positiveIntToByteString x) y) = Some (x, y)"
+  apply (cases y)
+  subgoal for ys
+    apply (simp only:byteStringToPositiveInt.simps appendByteStrings.simps positiveIntToByteString.simps)
+    using positiveIntToByteStringToPositiveIntAux by auto
+  done
+
+lemma byteStringToPositiveIntAuxIsPositive : "byteStringToPositiveIntAux x = Some (a, b) \<Longrightarrow> a \<ge> 0"
+  apply (induction x arbitrary:a b rule:byteStringToPositiveIntAux.induct)
+  apply simp
+  subgoal for xw rest a b
+    apply (cases "uint xw < 128")
+    apply auto
+    apply (cases "byteStringToPositiveIntAux rest")
+    by auto
+  done
+
+lemma byteStringToPositiveIntIsPositive : "byteStringToPositiveInt x = Some (a, b) \<Longrightarrow> a \<ge> 0"
+  apply (cases x)
+  subgoal sx
+  by (metis (no_types, lifting) byteStringToPositiveInt.simps byteStringToPositiveIntAuxIsPositive case_prod_conv option.distinct(1) option.exhaust option.inject option.simps(4) option.simps(5) prod.inject surj_pair)
+  done
+
+lemma unitRestoration : "a \<ge> 0 \<Longrightarrow> xh \<ge> 128 \<Longrightarrow> xh < 256 \<Longrightarrow> (xh + 128 * aaa) mod 128 + 128 = (xh :: int)"
+  apply simp
+  by (smt (z3) Euclidean_Division.pos_mod_bound mod_double_modulus mod_pos_pos_trivial)
+
+lemma inductiveStepInjection_aux : "Some (xh - 128 + 128 * (aaa + 1), aab) = Some (a, b) \<Longrightarrow> xh < 256 \<Longrightarrow> xh \<ge> (128 :: int) \<Longrightarrow>
+                                    byteStringToPositiveIntAux xt = Some (aaa, aab) \<Longrightarrow> a \<ge> 128 \<Longrightarrow> byteStringToPositiveIntAux xt = Some (a div 128 - 1, b)"
+  by auto
+
+lemma inductiveStepInjection_aux2 : "(\<And>a b. byteStringToPositiveIntAux xt = Some (a, b) \<Longrightarrow> positiveIntToByteStringAux a @ b = xt) \<Longrightarrow>
+    Some (uint (xh :: 8 word) - 128 + 128 * (aaa + 1), aab) = Some (a, b) \<Longrightarrow> uint xh \<ge> 128 \<Longrightarrow> byteStringToPositiveIntAux xt = Some aa \<Longrightarrow> aa = (aaa, aab) \<Longrightarrow> a \<ge> 128 \<Longrightarrow> positiveIntToByteStringAux (a div 128 - 1) @ b = xt"
+  subgoal premises fact
+    apply (rule fact(1))
+    apply (rule inductiveStepInjection_aux[of "uint xh" aaa aab a b xt])
+    using fact(2) apply blast
+  apply (cases "xh")
+       apply auto
+    subgoal for n2
+      by (metis intToWordToUint less_imp_of_nat_less of_int_of_nat_eq of_nat_0_le_iff of_nat_numeral)
+      apply (simp add: fact(3))
+     apply (simp add: fact(4) fact(5))
+    by (simp add: fact(6))
+  done
+
+lemma splitAnd1 : "b \<Longrightarrow> c \<Longrightarrow> b \<and> c"
+  by simp
+
+lemma splitAnd2 : "(a \<Longrightarrow> b) \<Longrightarrow> (a \<Longrightarrow> c) \<Longrightarrow> a \<longrightarrow> b \<and> c"
+  by simp
+
+lemma nat_mod_id : "(n :: nat) < 256 \<Longrightarrow> n mod 2 ^ 8 = n"
+  by auto
+
+lemma inductiveStepInjection : "(\<And>a b. byteStringToPositiveIntAux xt = Some (a, b) \<Longrightarrow> positiveIntToByteStringAux a @ b = xt) \<Longrightarrow>
+    Some (uint xh - 128 + 128 * (aaa + 1), aab) = Some (a, b) \<Longrightarrow>
+    \<not> uint (xh :: 8 word) < 128 \<Longrightarrow> byteStringToPositiveIntAux xt = Some aa \<Longrightarrow> aa = (aaa, aab) \<Longrightarrow> (a < 128 \<longrightarrow> word_of_int a = xh \<and> b = xt) \<and> (\<not> a < 128 \<longrightarrow> word_of_int (a mod 128 + 128) = xh \<and> positiveIntToByteStringAux (a div 128 - 1) @ b = xt)"
+  apply (rule splitAnd1)
+  using byteStringToPositiveIntAuxIsPositive apply fastforce
+  apply (rule splitAnd2)
+   apply (cases "xh")
+  subgoal for n
+    apply auto[1]
+    by (metis fold_sig_bit_in_word_of_int intToWordToUint less_imp_of_nat_less mod_mult_self2 of_int_of_nat_eq of_nat_0_le_iff of_nat_numeral unitRestoration verit_comp_simplify1(3))
+  apply (rule inductiveStepInjection_aux2)
+  by auto
+
+lemma byteStrintToPositiveIntAux_inverseRoundtrip : "byteStringToPositiveIntAux x = Some (a, b) \<Longrightarrow> positiveIntToByteStringAux a @ b = x"
+  apply (induction x arbitrary:a b)
+   apply simp
+  subgoal for xh xt a b
+    apply (simp only:positiveIntToByteStringAux.simps[of a] byteStringToPositiveIntAux.simps)
+    apply (cases "uint xh < 128")
+     apply (simp del:positiveIntToByteStringAux.simps byteStringToPositiveIntAux.simps)
+    using word_of_int_uint apply blast
+     apply (simp del:positiveIntToByteStringAux.simps byteStringToPositiveIntAux.simps)
+    apply (cases "byteStringToPositiveIntAux xt")
+    apply simp
+    subgoal for aa
+      apply (cases aa)
+      subgoal for aaa aab
+        apply (subst fold_sig_bit_in_word_of_int)
+        apply (rule inductiveStepInjection)
+        by auto
+      done
+    done
+  done
+
+theorem byteStrintToPositiveInt_inverseRoundtrip : "byteStringToPositiveInt x = Some (a, b) \<Longrightarrow> appendByteStrings (positiveIntToByteString a) b = x"
+  apply (cases x)
+  apply (cases b)
+  subgoal for sx sb
+    apply (simp only:positiveIntToByteString.simps appendByteStrings.simps byteStringToPositiveInt.simps)
+    by (smt (verit, ccfv_SIG) byteStrintToPositiveIntAux_inverseRoundtrip case_prod_conv innerListByteString.simps not_None_eq option.collapse option.distinct(1) option.inject option.simps(4) option.simps(5) prod.inject surj_pair)
+  done
+
+lemma byteStringToPositiveInt_injective : "byteStringToPositiveInt x = Some (a, b) \<Longrightarrow> byteStringToPositiveInt y = Some (a, b) \<Longrightarrow> x = y"
+  using byteStrintToPositiveInt_inverseRoundtrip by blast
+
+lemma byteStringToPositiveInt_injective2 : "x \<noteq> y \<Longrightarrow> (byteStringToPositiveInt x \<noteq> byteStringToPositiveInt y) \<or> (byteStringToPositiveInt x = None) \<or> (byteStringToPositiveInt y = None)"
+  using byteStringToPositiveInt_injective by force
+
+fun intToByteString :: "int \<Rightarrow> ByteString" where
+"intToByteString x = (if x \<ge> 0 then positiveIntToByteString (x * 2) else positiveIntToByteString (- (x * 2 + 1)))"
+
+fun byteStringToInt :: "ByteString \<Rightarrow> (int \<times> ByteString) option" where
+"byteStringToInt x =
+  (case byteStringToPositiveInt x of
+     None \<Rightarrow> None
+   | Some (y, extra) \<Rightarrow> Some (if (y mod 2 = 0) then y div 2 else (- (y div 2 + 1)), extra))"
+
+theorem intToByteStringToInt : "byteStringToInt (appendByteStrings (intToByteString x) y) = Some (x, y)"
+  apply (cases x)
+  by (simp_all del:byteStringToPositiveInt.simps positiveIntToByteString.simps add:positiveIntToByteStringToPositiveInt)
+
+
+theorem byteStringToInt_inverseRoundtrip : "byteStringToInt x = Some (a, b) \<Longrightarrow> appendByteStrings (intToByteString a) b = x"
+  apply (simp only:byteStringToInt.simps intToByteString.simps)
+  apply (cases "byteStringToPositiveInt x")
+  apply simp
+  subgoal for aa
+    apply (cases aa)
+    subgoal for aaa aab
+      apply (auto simp del:byteStringToPositiveInt.simps positiveIntToByteString.simps simp add:byteStrintToPositiveInt_inverseRoundtrip)
+      apply (simp add: byteStringToPositiveIntIsPositive)
+      apply (smt byteStringToPositiveIntIsPositive)
+      by (metis add.commute byteStrintToPositiveInt_inverseRoundtrip diff_add_cancel minus_mod_eq_mult_div mult.commute)
+    done
+  done
+
+lemma byteStringToInt_injective : "byteStringToInt x = Some (a, b) \<Longrightarrow> byteStringToInt y = Some (a, b) \<Longrightarrow> x = y"
+  using byteStringToInt_inverseRoundtrip by blast
+
+lemma byteStringToInt_injective2 : "x \<noteq> y \<Longrightarrow> (byteStringToInt x \<noteq> byteStringToInt y) \<or> (byteStringToInt x = None) \<or> (byteStringToInt y = None)"
+  using byteStringToInt_injective by force
+
+fun packByteString :: "ByteString \<Rightarrow> ByteString" where
+"packByteString bs = appendByteStrings (positiveIntToByteString (int (lengthByteString bs))) bs"
+
+fun getByteString :: "ByteString \<Rightarrow> (ByteString \<times> ByteString) option" where
+"getByteString bs =
+  (case byteStringToPositiveInt bs of
+     Some (val, rest) \<Rightarrow> if int (lengthByteString rest) < val
+                         then None
+                         else Some (takeByteString (nat val) rest, dropByteString (nat val) rest)
+   | None \<Rightarrow> None
+  )"
+
+lemma appendTakeByteStrings : "lengthByteString x = n \<Longrightarrow> takeByteString n (appendByteStrings x y) = x"
+  by (metis appendByteStrings.elims append_eq_conv_conj lengthByteString.simps takeByteString.simps)
+
+lemma appendDropByteStrings : "lengthByteString x = n \<Longrightarrow> dropByteString n (appendByteStrings x y) = y"
+  by (metis appendByteStrings.elims append_eq_conv_conj dropByteString.elims innerListByteString.simps lengthByteString.elims)
+
+lemma appendLength : "lengthByteString x + lengthByteString y = lengthByteString (appendByteStrings x y)"
+  apply (cases x)
+  apply (cases y)
+  by simp
+
+lemma addAndGetByteString : "getByteString (appendByteStrings (packByteString x) y) = Some (x, y)"
+  apply (simp only:getByteString.simps)
+  apply (cases "byteStringToPositiveInt (appendByteStrings (packByteString x) y)")
+  using appendByteStringsAssoc positiveIntToByteStringToPositiveInt apply force
+  subgoal for a
+    apply (simp only:option.cases)
+    apply (cases a)
+    subgoal for fa sa
+      apply (auto split:prod.split simp only:)
+      apply (cases "int (lengthByteString sa) < fa")
+       apply (simp only:if_True)
+  apply (smt (verit, del_insts) add.right_neutral add_mono_thms_linordered_semiring(1) appendByteStringsAssoc appendLength byteStrintToPositiveInt_inverseRoundtrip innerListByteString.elims le_zero_eq nat_int nat_le_eq_zle nat_le_linear of_nat_0_le_iff of_nat_0_le_iff of_nat_eq_iff option.inject packByteString.simps positiveIntToByteStringToPositiveInt prod.inject semiring_1_class.of_nat_0 split_nat)
+      using appendByteStringsAssoc appendDropByteStrings appendTakeByteStrings positiveIntToByteStringToPositiveInt by fastforce
+    done
+  done
+
+lemma resultOfTakeByteStringHasLength : "lengthByteString (takeByteString n x) = min n (lengthByteString x)"
+  by (metis innerListByteString.elims lengthByteString.simps length_take min.commute takeByteString.simps)
+
+lemma takeLengthIfLongEnough : "takeByteString n x = y \<Longrightarrow> lengthByteString x \<ge> n \<Longrightarrow> lengthByteString y = n" 
+  by (metis min.absorb1 resultOfTakeByteStringHasLength)
+
+lemma addAndGetByteString_inverseRoundtrip : "getByteString x = Some (y, z) \<Longrightarrow> appendByteStrings (packByteString y) z = x"
+  apply (simp only:getByteString.simps packByteString.simps split:option.splits prod.splits)
+   apply blast
+  subgoal for x2 x1 x2a
+    apply (cases "int (lengthByteString x2a) < x1")
+     apply (simp del:byteStringToPositiveInt.simps positiveIntToByteString.simps split:option.splits prod.splits)
+     apply (simp only:if_False)
+     apply (simp only:appendByteStringsAssoc)
+     thm byteStrintToPositiveInt_inverseRoundtrip[of x "int (lengthByteString y)" z]
+     apply (subst byteStrintToPositiveInt_inverseRoundtrip[of x "int (lengthByteString y)" "appendByteStrings y z"])
+     using appendTakeDropByteString byteStringToPositiveIntIsPositive takeLengthIfLongEnough apply force
+     by blast
+   done
+
+lemma byteStringToPositiveIntAux_reduceslist : "byteStringToPositiveIntAux x = Some (a, b) \<Longrightarrow>
+                                                    size b < size x"
+  apply (induction x rule:byteStringToPositiveIntAux.induct)
+  apply simp
+  subgoal for xw rest
+    apply (simp add:Let_def refl)
+    apply (cases "byteStringToPositiveIntAux rest")
+     apply (smt le_imp_less_Suc le_less option.distinct(1) option.inject option.simps(4) prod.inject)
+    subgoal for aa
+      apply (cases "uint xw < 128")
+       apply (auto split:prod.splits)
+      using byteStrintToPositiveIntAux_inverseRoundtrip by fastforce
+    done
+  done
+
+lemma byteStringToPositiveInt_reduceslist : "byteStringToPositiveInt x = Some (a, b) \<Longrightarrow>
+                                                    size b < size x"
+  apply (cases x)
+  apply (simp only:byteStringToPositiveInt.simps)
+  subgoal for sx
+    apply (cases "byteStringToPositiveIntAux sx")
+     apply simp
+    using byteStringToPositiveIntAux_reduceslist size_ByteString_overloaded_def by force
+  done
+
+lemma byteStringToInt_reduceslist : "byteStringToInt x = Some (a, b) \<Longrightarrow>
+                                                    size b < size x"
+  apply (cases x)
+  apply (simp only:byteStringToInt.simps)
+  subgoal for sx
+    apply (cases "byteStringToPositiveInt (ByteString sx)")
+     apply simp
+    subgoal for sxaa
+      apply (cases sxaa)
+      apply simp
+  using byteStringToPositiveInt.simps byteStringToPositiveInt_reduceslist by presburger
+  done
+  done
+
+lemma getByteString_reduceslist : "getByteString x = Some (a, b) \<Longrightarrow>
+                                                    size b < size x"
+  by (smt (verit, ccfv_threshold) addAndGetByteString_inverseRoundtrip add_diff_cancel_right' appendLength byteStringToPositiveInt_reduceslist cancel_comm_monoid_add_class.diff_cancel linorder_neqE_nat nat_int nat_zero_as_int not_add_less2 of_nat_0_le_iff of_nat_0_less_iff packByteString.simps positiveIntToByteStringToPositiveInt size_ByteString_overloaded_def)
+
+fun listToByteString_aux :: "('a \<Rightarrow> ByteString) \<Rightarrow> 'a list \<Rightarrow> ByteString" where
+"listToByteString_aux f (Cons h t) = appendByteStrings (f h) (listToByteString_aux f t)" |
+"listToByteString_aux f Nil = emptyByteString"
+
+fun listToByteString :: "('a \<Rightarrow> ByteString) \<Rightarrow> 'a list \<Rightarrow> ByteString" where
+"listToByteString f l = (let listLength = length l in appendByteStrings (positiveIntToByteString (int listLength)) (listToByteString_aux f l))"
+
+fun byteStringToList_aux :: "(ByteString \<Rightarrow> ('a \<times> ByteString) option) \<Rightarrow> int \<Rightarrow> ByteString \<Rightarrow> ('a list \<times> ByteString) option" where
+"byteStringToList_aux f n bs =
+  (if n > 0
+   then (case f bs of
+           None \<Rightarrow> None
+         | Some (a, nbs) \<Rightarrow> (case byteStringToList_aux f (n - 1) nbs of
+                               None \<Rightarrow> None
+                             | Some (lr, fbs) \<Rightarrow> Some (a # lr, fbs)))
+   else (Some (Nil, bs)))"
+
+fun byteStringToList :: "(ByteString \<Rightarrow> ('a \<times> ByteString) option) \<Rightarrow> ByteString \<Rightarrow> ('a list \<times> ByteString) option" where
+"byteStringToList f bs =
+  (case byteStringToPositiveInt bs of
+     None \<Rightarrow> None
+   | Some (listLength, nbs) \<Rightarrow> byteStringToList_aux f listLength nbs)"
+
+theorem listToByteStringTolist : "(\<And> x y. decode (appendByteStrings (encode x) y) = Some (x, y)) \<Longrightarrow> byteStringToList decode (appendByteStrings(listToByteString encode x) y) = Some (x, y)"
+  oops
+
+theorem byteStringToList_inverseRoundtrip : "(\<And> x a b. decode x = Some (a, b) \<Longrightarrow> appendByteStrings (encode a) b = x) \<Longrightarrow> byteStringToList decode x = Some (a, b) \<Longrightarrow> appendByteStrings (listToByteString encode a) b = x"
+  oops
+
+
+end
